tmp

int.v
@@ -1,13 +1,25 @@
-From mathcomp Require Import ssreflect seq ssrnat eqtype ssrbool ssrfun.
+From mathcomp Require Import ssreflect  ssrnat eqtype ssrbool ssrfun seq.
+
+Set Implicit Arguments.
+Unset Printing Implicit Defensive.
 
 Definition Atom  := nat.
 Definition Name  := nat.
 Definition FName := nat.
 
 Inductive Val := ATOM of Atom.
-Notation "'`' e" := (ATOM e) (at level 0).
+Notation "''' e" := (ATOM e) (at level 0).
 
 Inductive Var := VAR of Name.
+
+Definition eq_var  :=
+  fun '(VAR x) '(VAR y) => x == y.
+
+Lemma eqvarP : Equality.axiom eq_var.
+Proof. by case=> ?[?/=]; apply/(iffP eqP)=> [|[]]->. Qed.
+
+Canonical var_eqMixin := EqMixin eqvarP.
+Canonical var_eqType := Eval hnf in EqType Var var_eqMixin.
 
 Inductive Arg := 
   | Arg_Val of Val
@@ -15,10 +27,38 @@ Inductive Arg :=
 Coercion Arg_Val : Val >-> Arg.
 Coercion Arg_Var : Var >-> Arg.
 
+Definition eq_arg a b := 
+  match a, b with
+  | Arg_Val 'a, Arg_Val 'b => a == b
+  | Arg_Var (VAR x), Arg_Var (VAR y) => x == y
+  | _, _ => false
+  end.
+
+Lemma eqargP : Equality.axiom eq_arg.
+Proof. 
+  by case=> [][]?[][]?/=; try (by constructor); apply/(iffP eqP)=> [|[]]->. 
+Qed.
+
+Canonical arg_eqMixin := EqMixin eqargP.
+Canonical arg_eqType := Eval hnf in EqType Arg arg_eqMixin.
+
 Inductive Exp :=
   | Exp_Arg of Arg
   | CONS of Exp & Exp.
 Coercion Exp_Arg : Arg >-> Exp.
+
+Fixpoint eq_exp a b := 
+  match a, b with
+  | Exp_Arg a,  Exp_Arg b  => a == b
+  | CONS e1 e2, CONS e3 e4 => eq_exp e1 e4 && eq_exp e2 e4
+  | _,          _          => false
+  end.
+
+Lemma eqexpP : Equality.axiom eq_exp.
+Proof. Admitted.
+
+Canonical exp_eqMixin := EqMixin eqexpP.
+Canonical exp_eqType := Eval hnf in EqType Exp exp_eqMixin.
 
 Inductive Cntr :=
   | CONStest of Arg & Var & Var
@@ -27,14 +67,14 @@ Notation "'CONS?'" := (CONStest) (only parsing).
 Notation "'EQA?'"  := (ATOMtest) (only parsing).
 
 Inductive Tree := 
+  | RET  of Exp
   | LET  of Var  & Exp  & Tree
-  | COND of Cntr & Tree & Tree
-  | EXP  of Exp.
-Coercion EXP : Exp >-> Tree.
+  | COND of Cntr & Tree & Tree.
+Coercion RET : Exp >-> Tree.
 
-(*Inductive Def := DEFINE of FName & seq Var & Tree.*)
+Inductive Prog := DEFINE of FName & seq Var & Tree.
 
-Inductive Const :=
+(*Inductive Const :=
   | Const_Val of Val
   | CCONS of Const & Const.
 Coercion Const_Val : Val >-> Const.
@@ -42,23 +82,23 @@ Coercion Const_Val : Val >-> Const.
 Fixpoint ExpConst (e : Exp) : Const :=
   match e with
   | CONS e1 e2 => CCONS (ExpConst e1) (ExpConst e2)
-  | `a         => `a
-  | VAR a      => `a
+  | 'a         => 'a
+  | VAR a      => 'a
   end.
 
 Fixpoint ConstExp (c : Const) : Exp :=
   match c with
   | CCONS c1 c2 => CONS (ConstExp c1) (ConstExp c2)
-  | `a          => `a 
-  end.
+  | 'a          => 'a 
+  end.*)
 
-Inductive Bind := BIND of Var & Const.
-Notation "b ↦ c" := (BIND b c) (at level 100).
+Definition Bind := (Var * Exp)%type.
+Notation "b ↦ c" := (b, c) (at level 100).
 
 Definition Env := seq Bind.
 
 Definition getExp (b : Bind) : Exp := 
-  let: _ ↦ c := b in ConstExp c.
+  let: _ ↦ c := b in c.
 
 Definition ofind {T} a (s : seq T) := 
   ohead [seq x <- s | a x].
@@ -66,8 +106,149 @@ Definition ofind {T} a (s : seq T) :=
 Fixpoint subst (e : Exp) (env : Env) : Exp := 
   match e with 
   | CONS e1 e2 => CONS (subst e1 env) (subst e2 env)
-  | `a         => `a
-  | VAR a      => oapp getExp e (ofind (fun '(VAR b ↦ _) => a == b) env)
+  | 'a         => 'a
+  | VAR a      => head e [seq x.2 | x <- env & x.1 == VAR a]
   end.
 
-Notation "e /. env" := (subst e env) (at level 100).
+Notation "e '/s/' env" := (subst e env) (at level 0).
+
+Arguments subst : simpl never.
+
+Inductive Branch := 
+  | TRUE  of Env
+  | FALSE of Env.
+
+Definition cntr (c : Cntr) (e : Env) : Branch := 
+  match c with
+  | EQA? x y    => 
+    match x /s/ e, y /s/ e with
+    | Arg_Val 'a, Arg_Val 'b => if a == b then TRUE e else FALSE e
+    | _,   _ => FALSE e
+    end
+  | CONS? x h t => 
+    if x /s/ e is CONS a b then
+      TRUE ((h ↦ a) :: (t ↦ b) :: e)
+    else FALSE e
+  end.
+
+
+Fixpoint int (t : Tree) (e : Env) : Exp := 
+  match t with
+  | RET x         => subst x e
+  | LET v x t     => int t ((v ↦ x /s/ e) :: e)
+  | COND c t' t'' => 
+    match cntr c e with
+    | TRUE e'   => int t'  e'
+    | FALSE e'' => int t'' e''
+    end
+  end.
+
+Definition int_Prog (f : Prog) (e : seq Exp) := 
+  let: DEFINE _ vs t := f in
+  int t (zip vs e).
+
+Fixpoint FVExp (e : Exp) : seq Var := 
+  match e with
+  | CONS e1 e2 => FVExp e1 ++ FVExp e2
+  | VAR v      => [:: VAR v]
+  | _          => [::]
+  end.
+
+Definition closed e := FVExp e == [::].
+
+
+Definition FVArg (a : Arg) := 
+  if a is (Arg_Var x) then [:: x] else [::].
+
+
+Definition FVCntr (c : Cntr) : seq Var := 
+  match c with
+  | EQA? x y => FVArg x ++ FVArg y
+  | CONS? x h t => h :: t :: FVArg x
+  end.
+
+Fixpoint FVTree (t : Tree) : seq Var :=
+  match t with
+  | RET e        => FVExp e
+  | LET v x t    => FVExp x ++ [seq fv <- FVTree t | fv != v ]
+  | COND c t1 t2 => FVCntr c ++ FVTree t1 ++ FVTree t2
+  end.
+
+Lemma closed_subs e env: 
+  {subset FVExp e <= [seq i.1 | i <- env]} -> all closed [seq x.2 | x <- env] -> closed e /s/ env.
+Proof.
+elim: e=> [[[]|[]]|]//=.
+- rewrite /subst=> n H /allP; apply.
+  elim: env H=> //= [/(_ (VAR n))|[]/=]; first (apply; by rewrite inE).
+  move=> ???; case: ifP=> //=; first by rewrite inE eq_refl.
+  rewrite inE => E  H S; rewrite H ?orbT // => ? /[dup] /S /[swap].
+  rewrite inE=> /eqP->; by rewrite inE eq_sym E.
+move=> ? IHe1 ? IHe2 S?.
+rewrite /subst/closed/= -size_eq0 size_cat addn_eq0 ?size_eq0 -/subst.
+apply/andP; split.
+- apply/IHe1=>// ? I; apply/S; by rewrite mem_cat I.
+- apply/IHe2=>// ? I; apply/S; by rewrite mem_cat I orbT.
+Qed.
+
+Lemma cntr_env_TRUE c env e: 
+  cntr c env = TRUE e -> all closed [seq x.2 | x <- env] -> 
+  all closed [seq x.2 | x <- e] * subseq env e.
+Proof.
+case: c=> [/= a v u |/=??].
+- case: a; rewrite /subst=> [[]]; first move=> []//.
+  move=> n; case E : ([seq x.2 | x <- env & x.1 == VAR n])=> [|h l] //=.
+  move: E=> /[swap]; case: h=> // a b [<-].
+  rewrite (subseq_trans (subseq_cons env (u ↦ b))) ?subseq_cons //= => E.
+  move=> /[dup] A; move: (mem_head (CONS a b) l); rewrite -E=> /mapP[[/= ??]].
+  rewrite mem_filter/= => /andP[? /[swap]<-] /(map_f snd) H /allP/(_ _ H).
+  move=> /=; rewrite A /closed/= -size_eq0 size_cat addn_eq0 ?size_eq0.
+  by case/andP=>->->.
+case: (_ /s/ _)=> // [[]]// []?; case: (_ /s/ _)=> // [[]] // []?.
+case: ifP=> // ? [->]->; by rewrite subseq_refl.
+Qed.
+
+Lemma cntr_env_FALSE c env e: 
+  cntr c env = FALSE e -> e == env.
+Proof.
+case: c=> [/= >|/= ??]; case (_ /s/ _)=> //; first by move=> ?[->].
+2: by move=> ?? [->].
+case=> [[]|?[->]]//; case: (_ /s/ _)=> [[[]??|??[->]]|???[->]]//.
+by case:ifP=> // ?[->].
+Qed.
+
+Lemma closed_int t e: 
+  {subset FVTree t <= map fst e} -> all closed (map snd e) ->
+  closed (int t e).
+Proof.
+elim: t e => [|v > IHt ? H C|] /=.
+- elim=> [[[]//|[]/= n e S /allP H]|/=]; first apply/H.
+  elim: e S {H}=> [/(_ (VAR n)) |]; first by apply; rewrite inE.
+  move=> []/= ???; rewrite/subst=> /=.
+  case: ifP=> /=; first by rewrite inE eq_refl.
+  rewrite inE => E  H S; rewrite H ?orbT // => ? /[dup] /S /[swap].
+  rewrite inE=> /eqP->; by rewrite inE eq_sym E.
+- rewrite /closed => ? IHt1 ? IHt2 ? S ?. 
+  rewrite /= -size_eq0 size_cat addn_eq0 ?size_eq0.
+  rewrite IHt1 /= ?IHt2 //= => ? I; apply S; by rewrite mem_cat I ?orbT.
+- rewrite IHt /= ?C ?andbT => //= => [x|].
+  - case: (boolP (x == v))=> [/eqP->|E I]; rewrite inE ?eq_refl //.
+    apply/orP; right; apply/H; by rewrite mem_cat mem_filter E I /= orbT.
+  apply/closed_subs=> //; rewrite /closed=> ? I; apply/H; by rewrite mem_cat I.
+move=> c ? IHt ? IHt1 e; case E: (cntr c e); move: E.
+- move/cntr_env_TRUE=> H S /H[? sub]; apply/IHt=> // x I.
+  apply/(mem_subseq (map_subseq _ sub))/S; by rewrite ?mem_cat I /= orbT.
+move/cntr_env_FALSE/eqP-> => S *; apply/IHt1=> // ? I; apply/S.
+by rewrite ?mem_cat I /= ?orbT.
+Qed.
+
+Theorem closed_int_Prog t vs f e: 
+  all closed e -> size vs = size e ->
+  closed (int_Prog (DEFINE f vs t) e).
+Proof. Admitted.
+
+
+
+
+
+
+
